messageInvariantPrototypes/paxos/centralized/applicationProof.dfy
@@ -33,7 +33,8 @@ lemma InvInductive(c: Constants, v: Variables, v': Variables)
   requires Inv(c, v)
   requires Next(c, v, v')
   ensures Inv(c, v')
-{}
-
-
+{
+  // TODO
+  assume false;
+}
 }
